provide a ghost switch to make two-state evolution proofs optional

steel/Zeta.Steel.Main.fst
@@ -23,8 +23,12 @@ module SA = Zeta.SeqAux
 
 module Loops = Steel.ST.Loops
 
+let lock_perm (b: Ghost.erased bool) : Tot perm =
+  if b then half else full_perm
+
 [@@ __reduce__]
 let thread_inv_predicate
+  (b: Ghost.erased bool)
   (t:V.thread_state_t)
   (mlogs:TLM.t)
   : M.thread_state_model -> vprop
@@ -33,46 +37,49 @@ let thread_inv_predicate
       `star`
     V.thread_state_inv t tsm
       `star`
-    TLM.tid_pts_to mlogs tsm.M.thread_id half tsm.M.processed_entries false
+    TLM.tid_pts_to mlogs tsm.M.thread_id (lock_perm b) tsm.M.processed_entries false
 
-let thread_inv (t: V.thread_state_t)
-               (mlogs: TLM.t)
+let thread_inv 
+  (b: Ghost.erased bool)
+  (t: V.thread_state_t)
+  (mlogs: TLM.t)
   : vprop
-  = exists_ (thread_inv_predicate t mlogs)
+  = exists_ (thread_inv_predicate b t mlogs)
 
 [@@CAbstractStruct]
 noeq
-type thread_state (mlogs:TLM.t) =
+type thread_state (b: Ghost.erased bool) (mlogs:TLM.t) =
 {
   tid: tid;
-  tsm: tsm:V.thread_state_t{V.thread_id tsm == tid};
-  lock : Lock.cancellable_lock (thread_inv tsm mlogs)
+  tsm: V.thread_state_t;
+  tsm_prf: squash (V.thread_id tsm == tid);
+  lock : Lock.cancellable_lock (thread_inv b tsm mlogs)
 }
 
-let all_threads_t (mlogs:TLM.t) =
-  larray (thread_state mlogs) n_threads
+let all_threads_t (b: Ghost.erased bool) (mlogs:TLM.t) =
+  larray (thread_state b mlogs) n_threads
 
 noeq
-type top_level_state = {
+type top_level_state (b: Ghost.erased bool) = {
   aeh: AEH.aggregate_epoch_hashes;
-  all_threads : all_threads_t aeh.mlogs
+  all_threads : all_threads_t b aeh.mlogs
 }
 
-let tid_positions_ok #l (all_threads: Seq.seq (thread_state l))
+let tid_positions_ok (#b: Ghost.erased bool) #l (all_threads: Seq.seq (thread_state b l))
   : prop
   = forall (i:SA.seq_index all_threads).
         let si = Seq.index all_threads i in
         U16.v si.tid == i
 
 [@@__reduce__]
-let core_inv0 (t:top_level_state)
+let core_inv0 (#b: Ghost.erased bool) (t:top_level_state b)
   : vprop
   = exists_ (fun perm ->
     exists_ (fun v ->
       A.pts_to t.all_threads perm v `star`
       pure (tid_positions_ok v)))
 
-let core_inv (t:top_level_state)
+let core_inv t
   : vprop
   = core_inv0 t
 
@@ -95,12 +102,17 @@ let core_inv_gather t =
   rewrite (core_inv0 t) (core_inv t)
 
 [@@__steel_reduce__; __reduce__]
-let all_logs (t:top_level_state) (tlm:tid_log_map)
+let all_logs' (#b: Ghost.erased bool) (t:top_level_state b) (tlm:tid_log_map)
   : vprop
-  = TLM.tids_pts_to t.aeh.mlogs half tlm false
+  = TLM.tids_pts_to t.aeh.mlogs (lock_perm b) tlm false
 
 [@@__steel_reduce__; __reduce__]
-let log_of_tid (t:top_level_state) (tid:tid) (l:M.log)
+let all_logs (t:top_level_state true) (tlm:tid_log_map)
+  : vprop
+= all_logs' t tlm
+
+[@@__steel_reduce__; __reduce__]
+let log_of_tid (t:top_level_state true) (tid:tid) (l:M.log)
   : vprop
   = TLM.tid_pts_to t.aeh.mlogs tid half l false
 
@@ -108,38 +120,19 @@ let all_logs_log_of_tid t m tid _ =
   TLM.take_tid t.aeh.mlogs m tid
 
 [@@__steel_reduce__; __reduce__]
-let frozen_logs t m =
-  exists_ (fun p ->
-    TLM.tids_pts_to t.aeh.mlogs p m false
-  )
-
-let freeze_all_logs t m =
-  noop ()
-
-let frozen_logs_share t m =
-  let p = elim_exists () in
-  TLM.share_tids_pts_to _ _;
-  noop ()
-
-let frozen_logs_gather t m =
-  let p1 = elim_exists () in
-  let p2 = elim_exists () in
-  TLM.gather_tids_pts_to #_ #p1 #p2 _ m;
-  noop ()
-
-[@@__steel_reduce__; __reduce__]
-let snapshot (t:top_level_state) (tlm:tid_log_map)
+let snapshot (#b: Ghost.erased bool) (t:top_level_state b) (tlm:tid_log_map)
   : vprop
   = TLM.global_snapshot t.aeh.mlogs tlm
   
 let init_thread_state
   (#m:Ghost.erased (TLM.repr))
+  (b: Ghost.erased bool)
   (mlogs:TLM.t)
   (i:tid)
   (_:squash (Map.sel m i == Some Seq.empty))
-  : ST (thread_state mlogs)
-       (TLM.tids_pts_to mlogs half m false)
-       (fun st -> TLM.tids_pts_to mlogs half (Map.upd m i None) false)
+  : ST (thread_state b mlogs)
+       (TLM.tids_pts_to mlogs (lock_perm b) m false)
+       (fun st -> TLM.tids_pts_to mlogs (lock_perm b) (Map.upd m i None) false)
        (requires True)
        (ensures fun st -> st.tid == i)
   = let st = VerifierSteps.create i in
@@ -148,19 +141,19 @@ let init_thread_state
       (TLM.tid_pts_to _ _ _ _ _)
       (TLM.tid_pts_to mlogs
                       (M.init_thread_state_model i).M.thread_id
-                      half
+                      (lock_perm b)
                       (M.init_thread_state_model i).M.processed_entries
                       false);
     intro_pure (~ (M.init_thread_state_model i).M.failed);
     intro_exists (M.init_thread_state_model i)
-                 (thread_inv_predicate st mlogs);
+                 (thread_inv_predicate b st mlogs);
     rewrite
-      (exists_ (thread_inv_predicate st mlogs))
-      (thread_inv st mlogs);
-    let lock = Lock.new_cancellable_lock (thread_inv st mlogs) in
-    return ({tid = i; tsm = st; lock = lock})
+      (exists_ (thread_inv_predicate b st mlogs))
+      (thread_inv b st mlogs);
+    let lock = Lock.new_cancellable_lock (thread_inv b st mlogs) in
+    return ({tid = i; tsm = st; tsm_prf = (); lock = lock})
 
-let tid_positions_ok_until #l (all_threads:Seq.seq (thread_state l)) (i:nat)
+let tid_positions_ok_until (#b: Ghost.erased bool) #l (all_threads:Seq.seq (thread_state b l)) (i:nat)
   : prop
   = forall (j:SA.seq_index all_threads).
       j < i ==> (let sj = Seq.index all_threads j in
@@ -168,16 +161,16 @@ let tid_positions_ok_until #l (all_threads:Seq.seq (thread_state l)) (i:nat)
 
 let rec init_all_threads_state
   (#m:Ghost.erased (TLM.repr))
+  (#b: Ghost.erased bool)
   (#mlogs:TLM.t)
-  (all_threads:all_threads_t mlogs)
+  (all_threads:all_threads_t b mlogs)
   (i:U16.t{U16.v i <= U32.v n_threads})
   : ST unit
-       (TLM.tids_pts_to mlogs half m false
+       (TLM.tids_pts_to mlogs (lock_perm b) m false
           `star`
         exists_ (fun s -> A.pts_to all_threads full_perm s
                          `star`
                        pure (tid_positions_ok_until s (U16.v i))))
-                   
        (fun _ -> exists_ (fun s -> A.pts_to all_threads full_perm s
                                `star`
                              pure (tid_positions_ok_until s (Seq.length s))))
@@ -186,11 +179,10 @@ let rec init_all_threads_state
   = let s = elim_exists () in
     A.pts_to_length all_threads s;
     elim_pure (tid_positions_ok_until s (U16.v i));
-    let b = FStar.Int.Cast.uint16_to_uint32 i = n_threads in
-    if b returns STT _ _ (fun _ -> exists_ (fun s -> A.pts_to all_threads full_perm s
+    let check = FStar.Int.Cast.uint16_to_uint32 i = n_threads in
+    if check returns STT _ _ (fun _ -> exists_ (fun s -> A.pts_to all_threads full_perm s
                                   `star`
                                 pure (tid_positions_ok_until s (Seq.length s))))
-
     then begin
       intro_pure (tid_positions_ok_until s (Seq.length s));
       drop (TLM.tids_pts_to _ _ _ _);
@@ -202,7 +194,7 @@ let rec init_all_threads_state
       return ()
     end
     else begin
-      let st = init_thread_state mlogs i () in
+      let st = init_thread_state b mlogs i () in
       A.write all_threads (FStar.Int.Cast.uint16_to_uint32 i) st;
       rewrite
         (A.pts_to all_threads full_perm (Seq.upd s (U32.v (FStar.Int.Cast.uint16_to_uint32 i)) st))
@@ -213,31 +205,34 @@ let rec init_all_threads_state
         (fun s -> A.pts_to all_threads full_perm s
                  `star`
                pure (tid_positions_ok_until s (U16.v (U16.add i 1us))));
-      init_all_threads_state #(Map.upd m i None) #mlogs all_threads (U16.add i 1us)
+      init_all_threads_state #(Map.upd m i None) #b #mlogs all_threads (U16.add i 1us)
     end
 
 let init_aux (#opened:_)
   (aeh:AEH.aggregate_epoch_hashes)
-  (all_threads:all_threads_t aeh.mlogs)
-  (t:top_level_state)
-  (s:Ghost.erased (Seq.seq (thread_state aeh.mlogs)))
+  (#b: Ghost.erased bool)
+  (all_threads:all_threads_t b aeh.mlogs)
+  (t:top_level_state b)
+  (s:Ghost.erased (Seq.seq (thread_state b aeh.mlogs)))
   : STGhost unit opened
       (pure (tid_positions_ok s)
          `star`
        A.pts_to all_threads full_perm s
-         `star`
-       TLM.tids_pts_to aeh.mlogs half (Map.const (Some Seq.empty)) false)
+      )
+//         `star`
+//       TLM.tids_pts_to aeh.mlogs half (Map.const (Some Seq.empty)) false)
       (fun _ -> core_inv t
-               `star`
-             TLM.tids_pts_to t.aeh.mlogs half (Map.const (Some Seq.empty)) false)
+      )
+//               `star`
+//             TLM.tids_pts_to t.aeh.mlogs half (Map.const (Some Seq.empty)) false)
       (requires t.aeh == aeh /\ t.all_threads == all_threads)
       (ensures fun _ -> True)
   = rewrite (A.pts_to all_threads full_perm s)
             (A.pts_to t.all_threads full_perm s);
-    rewrite (TLM.tids_pts_to aeh.mlogs half (Map.const (Some Seq.empty)) false)
-            (TLM.tids_pts_to t.aeh.mlogs half (Map.const (Some Seq.empty)) false);
+//    rewrite (TLM.tids_pts_to aeh.mlogs half (Map.const (Some Seq.empty)) false)
+//            (TLM.tids_pts_to t.aeh.mlogs half (Map.const (Some Seq.empty)) false);
     rewrite (pure (tid_positions_ok s))
-            (pure (tid_positions_ok #(t.aeh.mlogs) s));
+            (pure (tid_positions_ok #b #(t.aeh.mlogs) s));
     intro_exists
       (Ghost.reveal s)
       (fun s -> A.pts_to t.all_threads full_perm s
@@ -250,10 +245,39 @@ let init_aux (#opened:_)
                                pure (tid_positions_ok s)));
     rewrite (exists_ _) (core_inv t)
 
-let init () =
+let share_tids_pts_to_post
+  (x: TLM.t)
+  (m: TLM.repr)
+  (b: Ghost.erased bool)
+: vprop
+= if b
+  then TLM.tids_pts_to x (lock_perm b) m false
+  else emp
+
+let share_tids_pts_to
+  (#o: _)
+  (x: TLM.t)
+  (m: TLM.repr)
+  (b: Ghost.erased bool)
+: STGhostT unit o
+  (TLM.tids_pts_to x full_perm m false)
+  (fun _ -> TLM.tids_pts_to x (lock_perm b) m false `star`
+     share_tids_pts_to_post x m b
+  )
+= if b
+  then begin
+    TLM.share_tids_pts_to x m;
+    rewrite (TLM.tids_pts_to x _ m false `star` TLM.tids_pts_to x _ m false)
+      (TLM.tids_pts_to x (lock_perm b) m false `star` share_tids_pts_to_post x m b)
+  end else begin
+    rewrite (TLM.tids_pts_to x _ m false) (TLM.tids_pts_to x (lock_perm b) m false);
+    rewrite emp (share_tids_pts_to_post x m b)
+  end
+
+let init b =
   let aeh = AEH.create () in
-  TLM.share_tids_pts_to aeh.mlogs (Map.const (Some Seq.empty));
-  let st0 = init_thread_state aeh.mlogs 0us () in
+  share_tids_pts_to aeh.mlogs (Map.const (Some Seq.empty)) b;
+  let st0 = init_thread_state b aeh.mlogs 0us () in
   let all_threads = A.alloc st0 n_threads in
   intro_pure (tid_positions_ok_until (Seq.create (U32.v n_threads) st0) 1);
   intro_exists
@@ -263,6 +287,7 @@ let init () =
            pure (tid_positions_ok_until s 1));
   init_all_threads_state
     #(Map.upd (Map.const (Some Seq.empty)) 0us None)
+    #b
     #aeh.mlogs
     all_threads
     1us;
@@ -276,13 +301,108 @@ let init () =
   let r = ({ aeh = aeh; all_threads = all_threads }) in
   init_aux aeh all_threads r s;
   let t = R.alloc r in
-  intro_exists r (fun ts ->
-    R.pts_to t full ts `star`
-    core_inv ts `star`
-    all_logs ts (Map.const (Some Seq.empty)));
+  rewrite (share_tids_pts_to_post _ _ _) (init_post r);
   return t
 
-let verify_log_aux (t:top_level_state)
+let exists_log_of_tid_gen_intro
+  (#opened: _)
+  (#b: Ghost.erased bool)
+  (t: top_level_state b)
+  (tid: tid)
+  (entries: AEH.log)
+: STGhostT unit opened
+    (log_of_tid_gen t tid entries)
+    (fun _ -> exists_log_of_tid_gen t tid)
+= if b returns STGhostT unit opened
+    (log_of_tid_gen t tid entries)
+    (fun _ -> exists_log_of_tid_gen t tid)
+  then begin
+    rewrite (log_of_tid_gen t tid entries) (log_of_tid t tid entries);
+    rewrite (exists_log_of_tid t tid) (exists_log_of_tid_gen t tid)
+  end else begin
+    rewrite (log_of_tid_gen t tid entries) (exists_log_of_tid_gen t tid)
+  end
+
+inline_for_extraction
+noextract
+let steel_ifthenelse
+  (#t: Type)
+  (#vpre: vprop)
+  (#vpost: (t -> vprop))
+  (b: bool)
+  (ttrue: (squash (b == true) -> STT t vpre vpost))
+  (tfalse: (squash (b == false) -> STT t vpre vpost))
+: STF t vpre vpost True (fun _ -> True)
+= if b then ttrue () else tfalse ()
+
+inline_for_extraction
+noextract
+let steel_ifthenelse_not
+  (#t: Type)
+  (#vpre: vprop)
+  (#vpost: (t -> vprop))
+  (b: bool)
+  (tfalse: (squash (b == false) -> STT t vpre vpost))
+  (ttrue: (squash (b == true) -> STT t vpre vpost))
+: STF t vpre vpost True (fun _ -> True)
+= if b then ttrue () else tfalse ()
+
+#set-options "--print_implicits"
+
+let fake_vprop : vprop = pure False
+
+let fake_fail (#t: Type) (#pre: vprop) (#p: (t -> vprop)) () : STF t (pre `star` fake_vprop) p True (fun _ -> True) =
+  rewrite fake_vprop (pure False);
+  elim_pure False;
+  let res = false_elim #t () in
+  rewrite pre (p res);
+  return res
+
+let gather_thread_logs
+  (#opened: _)
+  (incremental: Ghost.erased bool)
+  (t: top_level_state incremental)
+  (tid: tid)
+  (entries1 entries2: AEH.log)
+: STGhost unit opened
+    (TLM.tid_pts_to t.aeh.mlogs tid (lock_perm incremental) entries1 false `star`
+      log_of_tid_gen #incremental t tid entries2)
+    (fun _ -> TLM.tid_pts_to t.aeh.mlogs tid full entries1 false)
+    True
+    (fun _ -> Ghost.reveal incremental == true ==> entries1 == entries2)
+=
+  if incremental
+  then begin
+    rewrite (log_of_tid_gen _ _ _) (TLM.tid_pts_to t.aeh.mlogs tid half entries2 false);
+    TLM.gather_tid_pts_to #_ #_ #(lock_perm incremental) t.aeh.mlogs;
+    vpattern_rewrite (fun p -> TLM.tid_pts_to t.aeh.mlogs tid p entries1 false) full
+  end else begin
+    vpattern_rewrite (fun p -> TLM.tid_pts_to t.aeh.mlogs tid p entries1 false) full;
+    rewrite (log_of_tid_gen _ _ _) emp
+  end
+
+let share_thread_logs
+  (#opened: _)
+  (incremental: Ghost.erased bool)
+  (t: top_level_state incremental)
+  (tid: tid)
+  (entries: AEH.log)
+: STGhostT unit opened
+    (TLM.tid_pts_to t.aeh.mlogs tid full entries false)
+    (fun _ -> TLM.tid_pts_to t.aeh.mlogs tid (lock_perm incremental) entries false `star`
+      log_of_tid_gen #incremental t tid entries)
+= if incremental
+  then begin
+    TLM.share_tid_pts_to t.aeh.mlogs;
+    rewrite (TLM.tid_pts_to _ _ _ _ _) (log_of_tid_gen #incremental t tid entries);
+    vpattern_rewrite (fun p -> TLM.tid_pts_to _ _ p _ _) (lock_perm incremental)
+  end else begin
+    vpattern_rewrite (fun p -> TLM.tid_pts_to _ _ p _ _) (lock_perm incremental);
+    rewrite emp  (log_of_tid_gen #incremental t tid entries)
+  end
+
+let verify_log_aux (#incremental: Ghost.erased bool)
+                   (t:top_level_state incremental)
                    (tid:tid)
                    (#entries:erased AEH.log)
                    (#log_perm:perm)
@@ -292,57 +412,35 @@ let verify_log_aux (t:top_level_state)
                    (out_len: U32.t)
                    (#out_bytes:erased bytes)
                    (output:larray U8.t out_len)
- : STT (option (v:V.verify_result { V.verify_result_complete len v }))
+ : STT (option (verify_result len))
     (core_inv t `star`
      A.pts_to input log_perm log_bytes `star`
      A.pts_to output full_perm out_bytes `star`
-     log_of_tid t tid entries)
+     log_of_tid_gen t tid entries)
     (verify_post t tid entries log_perm log_bytes len input out_len out_bytes output)
- = rewrite (core_inv t)
-          (exists_ (fun perm -> exists_ (fun s ->
-           A.pts_to t.all_threads perm s
-             `star`
-           pure (tid_positions_ok s))));
+ = rewrite (core_inv t) (core_inv0 t);
   let perm = elim_exists () in
   let s = elim_exists () in
-  extract_pure (tid_positions_ok s);
+  let sq : squash (tid_positions_ok s) = elim_pure (tid_positions_ok s) in
 
   A.pts_to_length t.all_threads s;
-  let st_tid = A.read t.all_threads (FStar.Int.Cast.uint16_to_uint32 tid) in
+  let st_tid : thread_state incremental t.aeh.mlogs = A.read t.all_threads (FStar.Int.Cast.uint16_to_uint32 tid) in
 
-  let b = Lock.acquire st_tid.lock in
-  match b returns STT _
-                      (A.pts_to input log_perm log_bytes
-                         `star`
-                       A.pts_to output full_perm out_bytes
-                         `star`
-                       TLM.tid_pts_to _ _ _ _ _
-                         `star`
-                       A.pts_to t.all_threads perm s
-                         `star`
-                       pure (tid_positions_ok s)
-                         `star`
-                       Lock.maybe_acquired b st_tid.lock)
-                      (verify_post
-                         t
-                         tid
-                         entries
-                         log_perm
-                         log_bytes
-                         len
-                         input
-                         out_len
-                         out_bytes
-                         output) with
-  | false ->
+  let b = Lock.acquire #(thread_inv incremental st_tid.tsm t.aeh.mlogs) st_tid.lock in
+
+  steel_ifthenelse_not
+    b
+    (fun _ ->
     //
     //Acquiring the lock for this thread's local state failed
     //This indicates an earlier failure
     //Reestablish the inv. and return
     //
-    let r = None in
-    rewrite (Lock.maybe_acquired false st_tid.lock)
-            emp;
+
+    noop ();
+    let r : option (verify_result len) = None in
+    rewrite (Lock.maybe_acquired b st_tid.lock) emp;
+
     intro_exists (Ghost.reveal s)
                  (fun s -> A.pts_to t.all_threads perm s
                           `star`
@@ -359,9 +457,9 @@ let verify_log_aux (t:top_level_state)
     intro_exists
       (Ghost.reveal out_bytes)
       (fun s -> A.pts_to output full_perm s);
-    intro_exists
-      (Ghost.reveal entries)
-      (fun entries -> log_of_tid t tid entries);
+
+    exists_log_of_tid_gen_intro t tid entries;
+    
     rewrite
       (core_inv t
          `star`
@@ -369,16 +467,21 @@ let verify_log_aux (t:top_level_state)
          `star`
        (exists_ (fun s -> A.pts_to output full_perm s)
           `star`
-        exists_ (fun entries -> log_of_tid t tid entries)))
+        exists_log_of_tid_gen t tid))
       (verify_post t tid entries log_perm log_bytes len input out_len out_bytes output r);
+
     return r
-  | _ ->
+    
+    )
+
+    (fun _ ->
+
     rewrite (Lock.maybe_acquired _ _)
-            (thread_inv st_tid.tsm t.aeh.mlogs
+            (thread_inv incremental st_tid.tsm t.aeh.mlogs
                `star`
              Lock.can_release st_tid.lock);
-    rewrite (thread_inv st_tid.tsm t.aeh.mlogs)
-            (exists_ (thread_inv_predicate st_tid.tsm t.aeh.mlogs));
+    rewrite (thread_inv incremental st_tid.tsm t.aeh.mlogs)
+            (exists_ (thread_inv_predicate incremental st_tid.tsm t.aeh.mlogs));
     let tsm = elim_exists () in
 
     elim_pure (~ tsm.M.failed);
@@ -386,14 +489,10 @@ let verify_log_aux (t:top_level_state)
     VerifierTypes.extract_tsm_entries_invariant st_tid.tsm;
 
     rewrite
-      (TLM.tid_pts_to t.aeh.mlogs tid half entries false)
-      (TLM.tid_pts_to t.aeh.mlogs tsm.M.thread_id half entries false);
+      (log_of_tid_gen #incremental t tid entries)
+      (log_of_tid_gen #incremental t tsm.M.thread_id entries);
 
-    TLM.gather_tid_pts_to #_ #_ #_ #_ #entries #tsm.M.processed_entries t.aeh.mlogs;
-  
-    rewrite
-      (TLM.tid_pts_to t.aeh.mlogs tsm.M.thread_id (sum_perm half half) tsm.M.processed_entries false)
-      (TLM.tid_pts_to t.aeh.mlogs tsm.M.thread_id full tsm.M.processed_entries false);
+    gather_thread_logs _ _ _ _ _;
 
     //
     //Call into the single-threaded verifier
@@ -401,31 +500,17 @@ let verify_log_aux (t:top_level_state)
 
     let vr = V.verify_log st_tid.tsm input output t.aeh in
 
-    match vr returns STT _
-                         (Lock.can_release _
-                            `star`
-                          (pure (tid_positions_ok _)
-                             `star`
-                           (A.pts_to t.all_threads _ _
-                              `star`
-                            (V.verify_post _ _ _ _ _ _ _
-                               `star`
-                             A.pts_to input _ _))))
-                         (verify_post
-                            t
-                            tid
-                            entries
-                            log_perm
-                            log_bytes
-                            len
-                            input
-                            out_len
-                            out_bytes
-                            output) with
-    | V.Verify_success read wrote ->
+    steel_ifthenelse (V.Verify_success? vr)
+
+    (fun _ ->
+
+      let V.Verify_success read wrote = vr in
+
       rewrite
         (V.verify_post _ _ _ _ _ _ _)
         (exists_ (V.verify_post_success_pred tsm st_tid.tsm log_bytes out_bytes output t.aeh read wrote));
+
+      
       let log = elim_exists () in
       M.verify_model_thread_id_inv tsm log;  //to get the following assertion about thread id
       assert ((M.verify_model tsm log).thread_id == tid);
@@ -438,13 +523,15 @@ let verify_log_aux (t:top_level_state)
       //
       let b_failed = VerifierSteps.check_failed st_tid.tsm in
 
-      if b_failed
-      then begin
+      steel_ifthenelse b_failed
+
+      (fun _ ->
         //
         //Similar to the case of lock failure,
         //  establish the invariant and return
         //
         Lock.cancel st_tid.lock;
+        
         intro_exists (Ghost.reveal s)
                      (fun s -> A.pts_to t.all_threads perm s
                               `star`
@@ -466,23 +553,10 @@ let verify_log_aux (t:top_level_state)
           (Ghost.reveal out_bytes1)
           (fun s -> A.pts_to output full_perm s);
 
-        TLM.share_tid_pts_to t.aeh.mlogs;
-        rewrite
-          (TLM.tid_pts_to
-             t.aeh.mlogs
-             (M.verify_model tsm log).thread_id
-             (half_perm full)
-             (M.verify_model tsm log).processed_entries
-             false)
-          (TLM.tid_pts_to
-             t.aeh.mlogs
-             tid
-             half
-             (M.verify_model tsm log).processed_entries
-             false);
-        intro_exists
-          ((M.verify_model tsm log).processed_entries)
-          (fun entries' -> log_of_tid t tid entries');
+        share_thread_logs _ _ _ _; 
+
+        vpattern_rewrite (fun tid -> log_of_tid_gen _ tid _) tid;
+        exists_log_of_tid_gen_intro _ _ _;
 
         drop (TLM.tid_pts_to _ _ _ _ _);
         drop (V.thread_state_inv _ _);
@@ -495,31 +569,24 @@ let verify_log_aux (t:top_level_state)
              `star`
            (exists_ (fun s -> A.pts_to output full_perm s)
               `star`
-            exists_ (fun entries -> log_of_tid t tid entries)))
+            exists_log_of_tid_gen t tid
+          ))
           (verify_post t tid entries log_perm log_bytes len input out_len out_bytes output res);
         return res
-      end
-      else begin
+      )
+
+
+      (fun _ -> 
+      
         //Now we know that all is well
         //
         assert (not (M.verify_model tsm log).M.failed);
-        TLM.share_tid_pts_to t.aeh.mlogs;
-        rewrite
-          (TLM.tid_pts_to
-             t.aeh.mlogs
-             (M.verify_model tsm log).thread_id
-             (half_perm full)
-             (M.verify_model tsm log).processed_entries
-             false)
-          (TLM.tid_pts_to
-             t.aeh.mlogs
-             (M.verify_model tsm log).thread_id
-             half
-             (M.verify_model tsm log).processed_entries
-             false);
+        share_thread_logs _ _ _ _;
+
         intro_pure (~ (M.verify_model tsm log).M.failed);
-        intro_exists (M.verify_model tsm log) (thread_inv_predicate st_tid.tsm   t.aeh.mlogs);
+        intro_exists (M.verify_model tsm log) (thread_inv_predicate incremental st_tid.tsm   t.aeh.mlogs);
         Lock.release st_tid.lock;
+
         intro_exists (Ghost.reveal s)
                      (fun s -> A.pts_to t.all_threads perm s
                               `star`
@@ -536,23 +603,17 @@ let verify_log_aux (t:top_level_state)
         let out_bytes' = elim_exists () in
         elim_pure _;
         elim_pure _;
-        assert (tsm.M.processed_entries == Ghost.reveal entries);
+        
+        assert (Ghost.reveal incremental == true ==> tsm.M.processed_entries == Ghost.reveal entries);
         M.verify_model_append tsm log;
-        assert ((M.verify_model tsm log).processed_entries == Seq.append entries log);
+        assert ((M.verify_model tsm log).processed_entries == Seq.append tsm.M.processed_entries log);
+        
         rewrite
-          (TLM.tid_pts_to
-             t.aeh.mlogs
-             (M.verify_model tsm log).thread_id
-             (half_perm full)
-             (M.verify_model tsm log).processed_entries
-             false)
-          (TLM.tid_pts_to
-             t.aeh.mlogs
-             tid
-             half
-             (entries `Seq.append` log)
-             false);
+          (log_of_tid_gen _ _ _)
+          (log_of_tid_gen t tid (entries `Seq.append` log)); // works because if incremental == false, then both sides are emp
+
         intro_pure (verify_post_success_pure_inv
+                      incremental
                       tid
                       entries
                       log_bytes
@@ -561,6 +622,7 @@ let verify_log_aux (t:top_level_state)
                       wrote
                       (Ghost.reveal log)
                       out_bytes');
+
         intro_exists
           (Ghost.reveal out_bytes')
           (verify_post_success_out_bytes_pred t tid entries log_bytes out_len   out_bytes output read wrote log);
@@ -576,9 +638,11 @@ let verify_log_aux (t:top_level_state)
            exists_ (verify_post_success_pred t tid entries log_bytes out_len out_bytes output read wrote))
           (verify_post t tid entries log_perm log_bytes len input out_len out_bytes output res);
         return res
-      end
+      )
 
-    | _ ->
+    )
+
+    (fun _ ->
       //
       //Single-threaded verifier failed
       //
@@ -605,20 +669,13 @@ let verify_log_aux (t:top_level_state)
       elim_pure _;
       //drop thread_state_inv
       drop (exists_ (V.thread_state_inv st_tid.tsm));
+      
       let entries' = elim_exists #_ #_
         #(fun entries' -> TLM.tid_pts_to t.aeh.mlogs (V.thread_id st_tid.tsm) full entries' false)
         () in
-      rewrite
-        (TLM.tid_pts_to t.aeh.mlogs (V.thread_id st_tid.tsm) full entries' false)
-        (TLM.tid_pts_to t.aeh.mlogs tid full entries' false);
-      TLM.share_tid_pts_to t.aeh.mlogs;
-      drop (TLM.tid_pts_to t.aeh.mlogs tid (half_perm full) entries' false);
-      rewrite
-        (TLM.tid_pts_to t.aeh.mlogs tid (half_perm full) entries' false)
-        (TLM.tid_pts_to t.aeh.mlogs tid half entries' false);
-      intro_exists
-        (Ghost.reveal entries')
-        (fun entries' -> log_of_tid t tid entries');
+      share_thread_logs _ _ _ _;
+      drop (TLM.tid_pts_to _ _ _ _ _);
+      exists_log_of_tid_gen_intro _ _ _;
       let r = None in
       rewrite
         (core_inv t
@@ -627,48 +684,28 @@ let verify_log_aux (t:top_level_state)
            `star`
          (exists_ (fun s -> A.pts_to output full_perm s)
             `star`
-          exists_ (fun entries -> log_of_tid t tid entries)))
+          exists_log_of_tid_gen _ _
+         ))
         (verify_post t tid entries log_perm log_bytes len input out_len out_bytes output r);
       return r
 
-let verify_log (#p:perm)
-               (#t:erased top_level_state)
-               (r:R.ref top_level_state)
-               (tid:tid)
-               (#entries:erased AEH.log)
-               (#log_perm:perm)
-               (#log_bytes:erased bytes)
-               (len: U32.t { len <> 0ul })
-               (input:larray U8.t len)
-               (out_len: U32.t)
-               (#out_bytes:erased bytes)
-               (output:larray U8.t out_len)
-  : STT (option (v:V.verify_result { V.verify_result_complete len v }))
-    (R.pts_to r p t `star`
-     core_inv t `star`
-     A.pts_to input log_perm log_bytes `star`
-     A.pts_to output full_perm out_bytes `star`
-     log_of_tid t tid entries)
-    (fun res -> 
-       R.pts_to r p t `star`
-       verify_post t tid entries log_perm log_bytes len input out_len out_bytes output res)
+    )
+
+ )
+
+let verify_log
+  #p #b #t r tid #entries #log_perm #log_bytes len input out_len #out_bytes output
   = let t' = R.read r in
     rewrite (core_inv t) (core_inv t');
-    rewrite (log_of_tid t tid entries) (log_of_tid t' tid entries);
+    rewrite (log_of_tid_gen t tid entries) (log_of_tid_gen t' tid entries);
     let res = verify_log_aux t' tid len input out_len output in
     rewrite 
       (verify_post t' tid entries log_perm log_bytes len input out_len out_bytes output res)
       (verify_post t tid entries log_perm log_bytes len input out_len out_bytes output res);      
     return res
 
-let max_certified_epoch (#p:perm)
-                         (#t:erased top_level_state)
-                         (r:R.ref top_level_state)
-  : STT AEH.max_certified_epoch_result
-        (R.pts_to r p t)
-        (fun res -> 
-           R.pts_to r p t `star`
-           read_max_post t res)
+let max_certified_epoch
+  #p #b #t r
   = let t' = R.read r in
     let res = AEH.advance_and_read_max_certified_epoch t'.aeh in
     assert_ (AEH.read_max_post t'.aeh res);
